lean/RubyCore/Judgment/Json.lean
@@ -87,6 +87,7 @@ partial def derivToJson : Deriv → Json
        | none => []))
   | .defPromote b => Json.mkObj [("k", "defPromote"), ("body", derivToJson b)]
   | .classTop b => Json.mkObj [("k", "classTop"), ("body", derivToJson b)]
+  | .module' b => Json.mkObj [("k", "module"), ("body", derivToJson b)]
   | .sub d σ Γ'' =>
     Json.mkObj [("k", "sub"), ("d", derivToJson d), ("ty", tyToJson σ),
       ("env", envToJson Γ'')]
@@ -184,6 +185,7 @@ partial def derivOfJson (j : Json) : Except String Deriv := do
     pure (.defDecl ps ret bs (← derivOfJson (← j.getObjVal? "body")))
   | "defPromote" => pure (.defPromote (← derivOfJson (← j.getObjVal? "body")))
   | "classTop" => pure (.classTop (← derivOfJson (← j.getObjVal? "body")))
+  | "module" => pure (.module' (← derivOfJson (← j.getObjVal? "body")))
   | "sub" =>
     pure (.sub (← derivOfJson (← j.getObjVal? "d"))
       (← tyOfJson (← j.getObjVal? "ty")) (← envOfJson (← j.getObjVal? "env")))
